Merge

src/coq/Renaming.v
@@ -15,7 +15,10 @@ From ExtLib Require Import
      Programming.Eqv
      Structures.Monads.
 
-Require Import ITree.ITree.
+From ITree Require Import
+     ITree
+     Eq.Eq
+     Interp.TranslateFacts.
 
 From Vellvm Require Import 
      Error
@@ -29,533 +32,756 @@ From Vellvm Require Import
      Memory
      LLVMEvents.
 
-
-
-
 Import EqvNotation.
 
 Open Scope Z_scope.
 Open Scope string_scope.
 Open Scope eq_itree_scope.
 
-Module RENAMING
-       (A:MemoryAddress.ADDRESS)
-       (LLVMIO:LLVM_INTERACTIONS(A)).
+Set Nested Proofs Allowed.
 
-  Module SS := Denotation A LLVMIO.
-  Import SS.
-  Import LLVMIO.
-  
-Class Swap (A:Type) := swap : raw_id -> raw_id -> A -> A.
-
-Class SwapLaws (A:Type) `{Swap A} := {
-  swap_same_id :
-    forall (id:raw_id) (x:A), swap id id x = x;
-
-  swap_comm:
-    forall id1 id2 (x:A), swap id1 id2 x = swap id2 id1 x;
-
-  swap_swap_id :
-    forall id1 id2 (x:A), swap id1 id2 (swap id1 id2 x) = x
-}.
-
-Class SwapInvariant (A:Type) `{Swap A} := {
-  swap_invariant :
-    forall id1 id2 (x:A), swap id1 id2 x = x
-}.
-
-Definition swap_raw_id (id1 id2:raw_id) (id:raw_id) : raw_id :=
-  if id ~=? id1 then id2 else
-    if id ~=? id2 then id1 else
-      id.
-Instance swap_of_raw_id : Swap raw_id := swap_raw_id.
-Hint Unfold swap_of_raw_id.
-
-Ltac unfold_swaps :=
-  repeat match goal with
-         | [H : context [swap _ _ _] |- _] => unfold swap in H; autounfold in H
-         | [H : _ |- context[swap _ _ _] ] => unfold swap; autounfold
-         end.
-
-Ltac simpl_ifs :=
-  repeat match goal with
-         | [_ : context [if ?X then _ else _] |- _] => destruct (X)
-         | [_ : _ |- context [if ?X then _ else _ ]] => destruct (X)
-         end.
-
-Program Instance raw_id_swaplaws : SwapLaws raw_id.
-Next Obligation.
-  unfold_swaps. unfold swap_raw_id.
-  destruct (x ~=? id); auto.
-Qed.
-Next Obligation.
-  unfold_swaps. unfold swap_raw_id. simpl_ifs; subst; auto.
-  unfold eqv, eqv_raw_id in *. subst. reflexivity.
-Qed.
-Next Obligation.
-  unfold_swaps. unfold swap_raw_id. simpl_ifs; subst; unfold eqv, eqv_raw_id in *; subst; auto.
-  - contradiction.
-  - contradiction.
-  - contradiction.
-  - contradiction.
-Qed.    
-  
-
-Definition swap_ident (id1 id2:raw_id) (id:ident) : ident :=
-  match id with
-  | ID_Global i => ID_Global (swap id1 id2 i)
-  | ID_Local i => ID_Local (swap id1 id2 i)
-  end.
-Instance swap_of_ident : Swap ident := swap_ident.
-Program Instance ident_swaplaws : SwapLaws ident.
-Next Obligation.
-  unfold_swaps; unfold swap_of_ident; destruct x; simpl; rewrite swap_same_id; reflexivity.
-Qed.
-Next Obligation.
-  unfold_swaps; unfold swap_of_ident; destruct x; simpl; rewrite swap_comm; reflexivity.
-Qed.
-Next Obligation.
-  unfold_swaps; unfold swap_of_ident; destruct x; simpl; rewrite swap_swap_id; reflexivity.
-Qed.  
-
-
-Instance swap_of_pair {A B} `(SA:Swap A) `(SB:Swap B) : Swap (A * B)%type :=
-  fun id1 id2 p => (swap id1 id2 (fst p), swap id1 id2 (snd p)).
-Hint Unfold swap_of_pair.
-
-Program Instance swap_laws_pair {A B} `(SA:Swap A) `(SB:Swap B) `(SLA:SwapLaws A) `(SLB:SwapLaws B) : SwapLaws (A*B)%type.
-Next Obligation.
-  unfold swap. unfold swap_of_pair.
-  rewrite swap_same_id. rewrite swap_same_id. reflexivity.
-Qed.  
-Next Obligation.
-  unfold swap. unfold swap_of_pair. simpl.
-  rewrite swap_comm. rewrite (@swap_comm B) at 1. reflexivity. assumption.
-Qed.
-Next Obligation.
-  unfold swap. unfold swap_of_pair. simpl.
-  rewrite swap_swap_id. rewrite (@swap_swap_id B) at 1. reflexivity. assumption.
-Qed.
-
-Instance swap_of_option {A} `(SA:Swap A) : Swap (option A) :=
-  fun id1 id2 opt => match opt with None => None | Some x => Some (swap id1 id2 x) end.
-Hint Unfold swap_of_option.
-
-Instance swap_of_list {A} `(SA:Swap A) : Swap (list A) :=
-  fun id1 id2 l => List.map (swap id1 id2) l.
-Hint Unfold swap_of_list.
-
-Instance swap_of_err {A} `(SA:Swap A) : Swap (err A) :=
-  fun id1 id2 e =>
-    match e with 
-    | inl s => inl s
-    | inr a => inr (swap id1 id2 a)
-    end.
-Hint Unfold swap_of_err.
-
-Instance swap_of_bool : Swap bool :=
-  fun id1 id2 b => b.
-
-Instance swap_of_nat : Swap nat :=
-  fun id1 id2 n => n.
-
-Instance swap_of_int : Swap int :=
-  fun id1 id2 n => n.
-
-Instance swap_of_string : Swap string :=
-  fun id1 id2 s => s.
-
-Instance swap_of_ibinop : Swap ibinop :=
-  fun id1 id2 n => n.
-
-Instance swap_of_fbinop : Swap fbinop :=
-  fun id1 id2 n => n.
-
-Instance swap_of_icmp : Swap icmp :=
-  fun id1 id2 n => n.
-
-Instance swap_of_fcmp : Swap fcmp :=
-  fun id1 id2 n => n.
-
-Hint Unfold swap_of_bool swap_of_nat swap_of_string swap_of_int swap_of_ibinop swap_of_fbinop swap_of_icmp swap_of_fcmp.
-
-Fixpoint swap_typ (id1 id2:raw_id) (t:typ) : typ :=
-  match t with
-  | TYPE_Pointer t' => TYPE_Pointer (swap_typ id1 id2 t')
-  | TYPE_Array sz t' => TYPE_Array sz (swap_typ id1 id2 t')
-  | TYPE_Function ret args => TYPE_Function (swap_typ id1 id2 ret) (List.map (swap_typ id1 id2) args)
-  | TYPE_Struct fields => TYPE_Struct (List.map (swap_typ id1 id2) fields)
-  | TYPE_Packed_struct fields => TYPE_Packed_struct (List.map (swap_typ id1 id2) fields)
-  | TYPE_Vector sz t' => TYPE_Vector sz (swap_typ id1 id2 t')
-  | TYPE_Identified id => TYPE_Identified (swap id1 id2 id)
-  | _ => t
-  end.
-(* Hint Unfold swap_typ.*) (* DO WE WANT THESE UNFOLD HINTS? *)
-
-Instance swap_of_typ : Swap typ := swap_typ.
-Hint Unfold swap_of_typ.
-
-Instance swap_of_dtyp : Swap dtyp :=
-  fun id1 id2 d => d.
-
-Section WithT.
-  Variable T:Set.
-  Context `{ST: Swap T}.
-
-
-Instance swap_of_tident : Swap (tident T) := swap.
-Hint Unfold swap_of_tident.
-
-Fixpoint swap_exp (id1 id2:raw_id) (e:exp T) : exp T :=
-  match e with
-  | EXP_Ident id => EXP_Ident _ (swap id1 id2 id)
-  | EXP_Integer _
-  | EXP_Float   _
-  | EXP_Hex     _
-  | EXP_Bool    _
-  | EXP_Null
-  | EXP_Zero_initializer
-  | EXP_Cstring _
-  | EXP_Undef => e
-  | EXP_Struct fields =>
-    EXP_Struct _ (List.map (fun '(t,e) => (swap id1 id2 t, swap_exp id1 id2 e)) fields)
-  | EXP_Packed_struct fields =>
-    EXP_Packed_struct _ (List.map (fun '(t,e) => (swap id1 id2 t, swap_exp id1 id2 e)) fields)    
-  | EXP_Array elts =>
-    EXP_Array _ (List.map (fun '(t,e) => (swap id1 id2 t, swap_exp id1 id2 e)) elts)
-  | EXP_Vector elts =>
-    EXP_Vector _ (List.map (fun '(t,e) => (swap id1 id2 t, swap_exp id1 id2 e)) elts)
-  | OP_IBinop iop t v1 v2 =>
-    OP_IBinop _ (swap id1 id2 iop) (swap id1 id2 t) (swap_exp id1 id2 v1) (swap_exp id1 id2 v2)
-  | OP_ICmp cmp t v1 v2 =>
-    OP_ICmp _ (swap id1 id2 cmp) (swap id1 id2 t) (swap_exp id1 id2 v1) (swap_exp id1 id2 v2)
-  | OP_FBinop fop fm t v1 v2 =>
-    OP_FBinop _ (swap id1 id2 fop) fm (swap id1 id2 t) (swap_exp id1 id2 v1) (swap_exp id1 id2 v2)    
-  | OP_FCmp cmp t v1 v2 =>
-    OP_FCmp _ (swap id1 id2 cmp) (swap id1 id2 t) (swap_exp id1 id2 v1) (swap_exp id1 id2 v2)    
-  | OP_Conversion conv t_from v t_to =>
-    OP_Conversion _ conv (swap id1 id2 t_from) (swap_exp id1 id2 v) (swap id1 id2 t_to)
-  | OP_GetElementPtr t ptrval idxs =>
-    OP_GetElementPtr _ (swap id1 id2 t) (swap id1 id2 (fst ptrval), swap_exp id1 id2 (snd ptrval))
-                     (List.map (fun '(t,e) => (swap id1 id2 t, swap_exp id1 id2 e)) idxs)
-  | OP_ExtractElement vec idx =>
-    OP_ExtractElement _ (swap id1 id2 (fst vec), swap_exp id1 id2 (snd vec))
-                      (swap id1 id2 (fst idx), swap_exp id1 id2 (snd idx))
-  | OP_InsertElement  vec elt idx =>
-    OP_InsertElement _ (swap id1 id2 (fst vec), swap_exp id1 id2 (snd vec))
-                     (swap id1 id2 (fst elt), swap_exp id1 id2 (snd elt))                     
-                     (swap id1 id2 (fst idx), swap_exp id1 id2 (snd idx))
-  | OP_ShuffleVector vec1 vec2 idxmask =>
-    OP_ShuffleVector _ (swap id1 id2 (fst vec1), swap_exp id1 id2 (snd vec1))
-                     (swap id1 id2 (fst vec2), swap_exp id1 id2 (snd vec2))                     
-                     (swap id1 id2 (fst idxmask), swap_exp id1 id2 (snd idxmask))
-  | OP_ExtractValue  vec idxs =>
-    OP_ExtractValue  _ (swap id1 id2 (fst vec), swap_exp id1 id2 (snd vec))
-                     idxs
-  | OP_InsertValue vec elt idxs =>
-    OP_InsertValue _ (swap id1 id2 (fst vec), swap_exp id1 id2 (snd vec))
-                   (swap id1 id2 (fst elt), swap_exp id1 id2 (snd elt))
-                   idxs
-  | OP_Select cnd v1 v2 =>
-    OP_Select _ (swap id1 id2 (fst cnd), swap_exp id1 id2 (snd cnd))
-              (swap id1 id2 (fst v1), swap_exp id1 id2 (snd v1))
-              (swap id1 id2 (fst v2), swap_exp id1 id2 (snd v2))
-  end.
-
-Instance swap_of_exp : Swap (exp T) := swap_exp.
-Hint Unfold swap_of_exp.
-
-Definition swap_instr_id (id1 id2:raw_id) (i:instr_id) : instr_id :=
-  match i with
-  | IId id => IId (swap id1 id2 id)
-  | IVoid n => IVoid n  (* TODO: support renaming these too? *)
-  end.
-
-Instance swap_of_instr_id : Swap instr_id := swap_instr_id.
-Hint Unfold swap_of_instr_id.
-
-Definition swap_phi (id1 id2:raw_id) (p:phi T) : phi T :=
-  match p with
-  | Phi t args => Phi _ (swap id1 id2 t) (swap id1 id2 args)
-  end.
-Instance swap_of_phi : Swap (phi T) := swap_phi.
-Hint Unfold swap_of_phi.
-
-Definition swap_instr (id1 id2:raw_id) (ins:instr T) : instr T :=
-  match ins with
-  | INSTR_Op op => INSTR_Op _ (swap id1 id2 op)
-  | INSTR_Call fn args => INSTR_Call _ (swap id1 id2 fn) (swap id1 id2 args)
-  | INSTR_Alloca t nb align =>
-    INSTR_Alloca _ (swap id1 id2 t) (swap id1 id2 nb) align
-  | INSTR_Load volatile t ptr align =>
-    INSTR_Load _ volatile (swap id1 id2 t) (swap id1 id2 ptr) align
-  | INSTR_Store volatile val ptr align =>
-    INSTR_Store _ volatile (swap id1 id2 val) (swap id1 id2 ptr) align
-  | INSTR_Comment _
-  | INSTR_Fence
-  | INSTR_AtomicCmpXchg
-  | INSTR_AtomicRMW
-  | INSTR_Unreachable
-  | INSTR_VAArg
-  | INSTR_LandingPad => ins
-  end.
-Instance swap_of_instr : Swap (instr T) := swap_instr.
-Hint Unfold swap_of_instr.
-
-Definition swap_terminator (id1 id2:raw_id) (trm:terminator T) : terminator T :=
-  match trm with
-  | TERM_Ret  v => TERM_Ret _ (swap id1 id2 v)
-  | TERM_Ret_void => TERM_Ret_void _
-  | TERM_Br v br1 br2 => TERM_Br _ (swap id1 id2 v) (swap id1 id2 br1) (swap id1 id2 br2)
-  | TERM_Br_1 br => TERM_Br_1 _ (swap id1 id2 br)
-  | TERM_Switch  v default_dest brs =>
-    TERM_Switch _ (swap id1 id2 v) (swap id1 id2 default_dest) (swap id1 id2 brs)
-  | TERM_IndirectBr v brs =>
-    TERM_IndirectBr _ (swap id1 id2 v) (swap id1 id2 brs)
-  | TERM_Resume v => TERM_Resume _ (swap id1 id2 v)
-  | TERM_Invoke fnptrval args to_label unwind_label =>
-    TERM_Invoke _ (swap id1 id2 fnptrval) (swap id1 id2 args) (swap id1 id2 to_label) (swap id1 id2 unwind_label)
-  end.
-Instance swap_of_terminator : Swap (terminator T) := swap_terminator.
-Hint Unfold swap_of_terminator.
-
-Instance swap_of_param_attr : Swap param_attr :=
-  fun id1 id2 l => l.
-Instance swap_of_fn_attr : Swap fn_attr :=
-  fun id1 id2 l => l.
-Instance swap_of_cconv : Swap cconv :=
-  fun id1 id2 l => l.
-Instance swap_of_linkage : Swap linkage :=
-  fun id1 id2 l => l.
-Instance swap_of_visibility : Swap visibility :=
-    fun id1 id2 l => l.
-Instance swap_of_dll_storage : Swap dll_storage :=
-    fun id1 id2 l => l.
-Instance swap_of_thread_local_storage : Swap thread_local_storage :=
-  fun id1 id2 l => l.
-
-Hint Unfold swap_of_param_attr swap_of_fn_attr swap_of_cconv swap_of_linkage swap_of_visibility swap_of_dll_storage swap_of_thread_local_storage.
-
-Definition swap_global (id1 id2:raw_id) (g:global T) : (global T) :=
-  mk_global _
-      (swap id1 id2 (g_ident _ g))
-      (swap id1 id2 (g_typ _ g))     
-      (swap id1 id2 (g_constant _ g))
-      (swap id1 id2 (g_exp _ g))
-      (swap id1 id2 (g_linkage _ g))
-      (swap id1 id2 (g_visibility _ g))
-      (swap id1 id2 (g_dll_storage _ g))
-      (swap id1 id2 (g_thread_local _ g))
-      (swap id1 id2 (g_unnamed_addr _ g))
-      (swap id1 id2 (g_addrspace _ g))
-      (swap id1 id2 (g_externally_initialized _ g))
-      (swap id1 id2 (g_section _ g))
-      (swap id1 id2 (g_align _ g)).
-Hint Unfold swap_global.
-Instance swap_of_global : Swap (global T) := swap_global.
-Hint Unfold swap_of_global.
-
-Definition swap_declaration (id1 id2:raw_id) (d:declaration T) : declaration T :=
-  mk_declaration _
-    (swap id1 id2 (dc_name _ d))
-    (swap id1 id2 (dc_type _ d))
-    (swap id1 id2 (dc_param_attrs _ d))
-    (swap id1 id2 (dc_linkage _ d))
-    (swap id1 id2 (dc_visibility _ d))
-    (swap id1 id2 (dc_dll_storage _ d))
-    (swap id1 id2 (dc_cconv _ d))
-    (swap id1 id2 (dc_attrs _ d))
-    (swap id1 id2 (dc_section _ d))
-    (swap id1 id2 (dc_align _ d))
-    (swap id1 id2 (dc_gc _ d)).
-Hint Unfold swap_declaration.
-Instance swap_of_declaration : Swap (declaration T) := swap_declaration.    
-Hint Unfold swap_of_declaration.
-
-Definition swap_block (id1 id2:raw_id) (b:block T) : block T :=
-  mk_block _ (swap id1 id2 (blk_id _ b))
-           (swap id1 id2 (blk_phis _ b))
-           (swap id1 id2 (blk_code _ b))
-           (swap id1 id2 (blk_term _ b))
-           (blk_comments _ b).
-Hint Unfold swap_block.  
-Instance swap_of_block : Swap (block T) := swap_block.
-Hint Unfold swap_of_block.
-
-Definition swap_definition {FnBody:Set} `{SF: Swap FnBody} (id1 id2:raw_id) (d:definition T FnBody) : definition T FnBody :=
-  mk_definition _ _
-    (swap id1 id2 (df_prototype _ _ d))
-    (swap id1 id2 (df_args _ _ d))
-    (swap id1 id2 (df_instrs _ _ d)).
-Hint Unfold swap_definition.
-
-Instance swap_of_definition {FnBody:Set} `{SF:Swap FnBody} : Swap (definition T FnBody) :=
-  swap_definition.
-Hint Unfold swap_of_definition.
-
-
-Fixpoint swap_metadata (id1 id2:raw_id) (m:metadata T) : metadata T :=
-  match m with
-  | METADATA_Const  tv => METADATA_Const _ (swap id1 id2 tv)
-  | METADATA_Null => METADATA_Null _
-  | METADATA_Id id => METADATA_Id _ (swap id1 id2 id)
-  | METADATA_String str => METADATA_String _ (swap id1 id2 str)
-  | METADATA_Named strs => METADATA_Named _ (swap id1 id2 strs)
-  | METADATA_Node mds => METADATA_Node _ (List.map (swap_metadata id1 id2) mds)
-  end.
-Instance swap_of_metadata : Swap (metadata T) := swap_metadata.
-Hint Unfold swap_of_metadata.
-
-Definition swap_toplevel_entity {FnBody:Set} `{SF:Swap FnBody} (id1 id2:raw_id) (tle:toplevel_entity T FnBody) :=
-  match tle with
-  | TLE_Comment msg => tle
-  | TLE_Target tgt => TLE_Target _ _ (swap id1 id2 tgt)
-  | TLE_Datalayout layout => TLE_Datalayout _ _ (swap id1 id2 layout)
-  | TLE_Declaration decl => TLE_Declaration _ _ (swap id1 id2 decl)
-  | TLE_Definition defn => TLE_Definition _ _ (swap id1 id2 defn)
-  | TLE_Type_decl id t => TLE_Type_decl _ _ (swap id1 id2 id) (swap id1 id2 t)
-  | TLE_Source_filename s => TLE_Source_filename _ _ (swap id1 id2 s)
-  | TLE_Global g => TLE_Global _ _ (swap id1 id2 g)
-  | TLE_Metadata id md => TLE_Metadata _ _ (swap id1 id2 id) (swap id1 id2 md)
-  | TLE_Attribute_group i attrs => TLE_Attribute_group _ _ (swap id1 id2 i) (swap id1 id2 attrs)
-  end.
-
-Instance swap_of_toplevel_entity {FnBody:Set} `{SF:Swap FnBody} : Swap (toplevel_entity T FnBody) :=
-  swap_toplevel_entity.
-Hint Unfold swap_of_toplevel_entity.
-
-Definition swap_modul {FnBody:Set} `{SF:Swap FnBody} (id1 id2:raw_id) (m:modul T FnBody) : modul T FnBody :=
-  mk_modul _ _
-    (swap id1 id2 (m_name _ _ m))
-    (swap id1 id2 (m_target _ _ m))
-    (swap id1 id2 (m_datalayout _ _ m))
-    (swap id1 id2 (m_type_defs _ _ m))
-    (swap id1 id2 (m_globals _ _ m))
-    (swap id1 id2 (m_declarations _ _ m))
-    (swap id1 id2 (m_definitions _ _ m)).
-Hint Unfold swap_modul.
-
-Instance swap_of_modul {FnBody:Set} `{SF:Swap FnBody} : Swap (modul T FnBody) :=
-  swap_modul.
-Hint Unfold swap_of_modul.
-
-(*
-Definition swap_pc (id1 id2:raw_id) (p:pc) : pc :=
-  mk_pc (swap id1 id2 (fn p)) (swap id1 id2 (bk p)) (swap id1 id2 (pt p)).
-Hint Unfold swap_pc.
-
-Instance swap_of_pc : Swap pc := swap_pc.
-Hint Unfold swap_of_pc.
-
-Definition swap_cmd (id1 id2:raw_id) (c:cmd) : cmd :=
-  match c with
-  | Inst i => Inst (swap id1 id2 i)
-  | Term t => Term (swap id1 id2 t)
-  end.                    
-Instance swap_of_cmd : Swap cmd := swap_cmd.
-Hint Unfold swap_of_cmd.
-*)
-
-Definition swap_cfg (id1 id2:raw_id) (CFG:cfg T) : cfg T :=
-  mkCFG _ (swap id1 id2 (init _ CFG)) (swap id1 id2 (blks _ CFG)) (swap id1 id2 (args _ CFG)).
-Hint Unfold swap_cfg.
-
-Instance swap_of_cfg : Swap (cfg T) := swap_cfg.
-Hint Unfold swap_of_cfg.
-
-Instance swap_of_mcfg : Swap (mcfg T) := swap.
-Hint Unfold swap_of_mcfg.
-End WithT.
-
-Instance swap_of_inttyp : forall {x:Z}, Swap (inttyp x) := fun _ id1 id2 a => a.
-Instance swap_of_int1 : Swap int1 := fun id1 id2 a => a.
-Instance swap_of_int32 : Swap int32 := fun id1 id2 a => a.
-Instance swap_of_int64 : Swap int64 := fun id1 id2 a => a.
-Instance swap_of_ll_double : Swap ll_double := fun id1 id2 a => a.
-Instance swap_of_ll_float : Swap ll_float := fun id1 id2 a => a.
-Hint Unfold swap_of_inttyp swap_of_int1 swap_of_int32 swap_of_int64 swap_of_ll_double swap_of_ll_float.
-
-Instance swap_of_dvalue : Swap dvalue := fun (id1 id2 : raw_id) dv => dv.
-Hint Unfold swap_of_dvalue.
-
-Program Instance swap_invariant_dvalue_inst : SwapInvariant dvalue := _.
-Next Obligation.
-  constructor. intros. unfold swap. reflexivity.
-Defined.  
-
-Instance swap_of_IO X : Swap (MemoryE X) := fun id1 id2 x => x.
-Hint Unfold swap_of_IO.
-
-Definition swap_itree {X E} `{Swap X} (id1 id2:raw_id) (t:itree E X) : itree E X :=
-  ITree.map (swap id1 id2) t.
-  
-Instance swap_of_itree {X E} `{SX : Swap X} : Swap (itree E X) := swap_itree.
-Hint Unfold swap_of_itree.
-
-(*
-(* Parameter fold : forall A: Type, (key -> elt -> A -> A) -> t elt -> A -> A. *)
-(* Definition swap_ENV {X} `{SX : Swap X} (id1 id2:raw_id) (m:ENV.t X) : ENV.t X := *)
-(*   ENV.fold (fun k v n => ENV.add (swap id1 id2 k) (swap id1 id2 v) n) m (ENV.empty X). *)
-(* Hint Unfold swap_ENV. *)
-
-Instance swap_of_ENV {X} `{SX : Swap X} : Swap (ENV.t X) := swap_ENV.
-Hint Unfold swap_of_ENV.
+(** We define a renaming pass and prove it correct.
+    The basic operation consider is a _swap_ between two [raw_id].
  *)
 
+Module RENAMING
+       (A:MemoryAddress.ADDRESS)
+       (LLVMEvents:LLVM_INTERACTIONS(A)).
 
-(*
-Definition swap_frame (id1 id2:raw_id) (f:frame) : frame :=
-  match f with
-  | KRet e id q => KRet (swap id1 id2 e) (swap id1 id2 id) (swap id1 id2 q)
-  | KRet_void e q => KRet_void (swap id1 id2 e) (swap id1 id2 q)
-  end.
+  Module SS := Denotation A LLVMEvents.
+  Import SS.
+  Import LLVMEvents.
 
-Instance swap_of_frame : Swap frame := swap_frame.
-Hint Unfold swap_of_frame.
+  (******************** Type classes ********************)
 
-Definition swap_result (id1 id2:raw_id) (r:result) : result :=
-  match r with
-  | Done v => Done (swap id1 id2 v)
-  | Step s => Step (swap id1 id2 s)
-  end.       
+  (* Swap operation *)
+  Class Swap (A:Type) := swap : raw_id -> raw_id -> A -> A.
 
-Instance swap_of_result : Swap result := swap_result.
-Hint Unfold swap_of_result.
-*)
-Section PROOFS.
-(*
-  (* TODO: Add to Coq Library *)
-  Lemma Empty_Equals : forall {X} (e:ENV.t X), ENV.Empty e -> ENV.Equal (ENV.empty X) e.
-  Proof.
-    intros.
-    apply ENVFacts.Equal_mapsto_iff.
-    intros k x.
-    pose (H1 := H k x). clearbody H1.
-    split.
-    intros H2.
-    apply ENVFacts.empty_mapsto_iff in H2. contradiction.
-    intros. contradiction.
+  Class SwapLaws (A:Type) `{Swap A} :=
+    {
+      (* Swapping a variable for itself is the identity. *)
+      swap_same_id :
+        forall (id:raw_id) (x:A), swap id id x = x;
+
+      (* [swap] is commutative *)
+      swap_comm:
+        forall id1 id2 (x:A), swap id1 id2 x = swap id2 id1 x;
+
+      (* [swap] is idempotent *)
+      swap_swap_id :
+        forall id1 id2 (x:A), swap id1 id2 (swap id1 id2 x) = x
+    }.
+
+  (* Particular case where [swap] is [id] *)
+  Class SwapInvariant (A:Type) `{Swap A} :=
+    {
+      swap_invariant :
+        forall id1 id2 (x:A), swap id1 id2 x = x
+    }.
+
+  (******************** Swap instances ********************)
+
+  (******************** Syntactic swaps ********************)
+
+  Definition swap_raw_id (id1 id2:raw_id) (id:raw_id) : raw_id :=
+    if id ~=? id1 then id2 else
+      if id ~=? id2 then id1 else
+        id.
+  Instance swap_of_raw_id : Swap raw_id := swap_raw_id.
+  Hint Unfold swap_of_raw_id.
+
+  Ltac unfold_swaps :=
+    repeat match goal with
+           | [H : context [swap _ _ _] |- _] => unfold swap in H; autounfold in H
+           | [H : _ |- context[swap _ _ _] ] => unfold swap; autounfold
+           end.
+
+  Ltac simpl_ifs :=
+    repeat match goal with
+           | [_ : context [if ?X then _ else _] |- _] => destruct (X)
+           | [_ : _ |- context [if ?X then _ else _ ]] => destruct (X)
+           end.
+
+  Program Instance raw_id_swaplaws : SwapLaws raw_id.
+  Next Obligation.
+    unfold_swaps. unfold swap_raw_id.
+    destruct (x ~=? id); auto.
+  Qed.
+  Next Obligation.
+    unfold_swaps. unfold swap_raw_id. simpl_ifs; subst; auto.
+    unfold eqv, eqv_raw_id in *. subst. reflexivity.
+  Qed.
+  Next Obligation.
+    unfold_swaps. unfold swap_raw_id. simpl_ifs; subst; unfold eqv, eqv_raw_id in *; subst; auto.
+    - contradiction.
+    - contradiction.
+    - contradiction.
+    - contradiction.
+  Qed.    
+
+  Definition swap_ident (id1 id2:raw_id) (id:ident) : ident :=
+    match id with
+    | ID_Global i => ID_Global (swap id1 id2 i)
+    | ID_Local i => ID_Local (swap id1 id2 i)
+    end.
+  Instance swap_of_ident : Swap ident := swap_ident.
+  Program Instance ident_swaplaws : SwapLaws ident.
+  Next Obligation.
+    unfold_swaps; unfold swap_of_ident; destruct x; simpl; rewrite swap_same_id; reflexivity.
+  Qed.
+  Next Obligation.
+    unfold_swaps; unfold swap_of_ident; destruct x; simpl; rewrite swap_comm; reflexivity.
+  Qed.
+  Next Obligation.
+    unfold_swaps; unfold swap_of_ident; destruct x; simpl; rewrite swap_swap_id; reflexivity.
+  Qed.  
+
+  Instance swap_of_pair {A B} `(SA:Swap A) `(SB:Swap B) : Swap (A * B)%type :=
+    fun id1 id2 p => (swap id1 id2 (fst p), swap id1 id2 (snd p)).
+  Hint Unfold swap_of_pair.
+
+  Program Instance swap_laws_pair {A B} `(SA:Swap A) `(SB:Swap B) `(SLA:SwapLaws A) `(SLB:SwapLaws B) : SwapLaws (A*B)%type.
+  Next Obligation.
+    unfold swap. unfold swap_of_pair.
+    rewrite swap_same_id. rewrite swap_same_id. reflexivity.
+  Qed.  
+  Next Obligation.
+    unfold swap. unfold swap_of_pair. simpl.
+    rewrite swap_comm. rewrite (@swap_comm B) at 1. reflexivity. assumption.
+  Qed.
+  Next Obligation.
+    unfold swap. unfold swap_of_pair. simpl.
+    rewrite swap_swap_id. rewrite (@swap_swap_id B) at 1. reflexivity. assumption.
   Qed.
 
-  (* TODO: Add to Coq Library *)
-  Lemma find_Empty_none : forall {X} (e:ENV.t X) (id:raw_id), ENV.Empty e -> ENV.find id e = None.
+  Instance swap_of_option {A} `(SA:Swap A) : Swap (option A) :=
+    fun id1 id2 opt => match opt with None => None | Some x => Some (swap id1 id2 x) end.
+  Hint Unfold swap_of_option.
+
+  Instance swap_of_list {A} `(SA:Swap A) : Swap (list A) :=
+    fun id1 id2 l => List.map (swap id1 id2) l.
+  Hint Unfold swap_of_list.
+
+  Instance swap_of_err {A} `(SA:Swap A) : Swap (err A) :=
+    fun id1 id2 e =>
+      match e with 
+      | inl s => inl s
+      | inr a => inr (swap id1 id2 a)
+      end.
+  Hint Unfold swap_of_err.
+
+  Instance swap_of_bool : Swap bool :=
+    fun id1 id2 b => b.
+
+  Instance swap_of_nat : Swap nat :=
+    fun id1 id2 n => n.
+
+  Instance swap_of_int : Swap int :=
+    fun id1 id2 n => n.
+
+  Instance swap_of_string : Swap string :=
+    fun id1 id2 s => s.
+
+  Instance swap_of_ibinop : Swap ibinop :=
+    fun id1 id2 n => n.
+
+  Instance swap_of_fbinop : Swap fbinop :=
+    fun id1 id2 n => n.
+
+  Instance swap_of_icmp : Swap icmp :=
+    fun id1 id2 n => n.
+
+  Instance swap_of_fcmp : Swap fcmp :=
+    fun id1 id2 n => n.
+
+  Hint Unfold swap_of_bool swap_of_nat swap_of_string swap_of_int swap_of_ibinop swap_of_fbinop swap_of_icmp swap_of_fcmp.
+
+  Fixpoint swap_typ (id1 id2:raw_id) (t:typ) : typ :=
+    match t with
+    | TYPE_Pointer t' => TYPE_Pointer (swap_typ id1 id2 t')
+    | TYPE_Array sz t' => TYPE_Array sz (swap_typ id1 id2 t')
+    | TYPE_Function ret args => TYPE_Function (swap_typ id1 id2 ret) (List.map (swap_typ id1 id2) args)
+    | TYPE_Struct fields => TYPE_Struct (List.map (swap_typ id1 id2) fields)
+    | TYPE_Packed_struct fields => TYPE_Packed_struct (List.map (swap_typ id1 id2) fields)
+    | TYPE_Vector sz t' => TYPE_Vector sz (swap_typ id1 id2 t')
+    | TYPE_Identified id => TYPE_Identified (swap id1 id2 id)
+    | _ => t
+    end.
+  (* Hint Unfold swap_typ.*) (* DO WE WANT THESE UNFOLD HINTS? *)
+
+  Instance swap_of_typ : Swap typ := swap_typ.
+  Hint Unfold swap_of_typ.
+
+  Instance swap_of_dtyp : Swap dtyp :=
+    fun id1 id2 d => d.
+
+  Section WithT.
+    Variable T:Set.
+    Context `{ST: Swap T}.
+
+    Global Instance swap_of_tident : Swap (tident T) := swap.
+    Hint Unfold swap_of_tident.
+
+    Fixpoint swap_exp (id1 id2:raw_id) (e:exp T) : exp T :=
+      match e with
+      | EXP_Ident id => EXP_Ident _ (swap id1 id2 id)
+      | EXP_Integer _
+      | EXP_Float   _
+      | EXP_Hex     _
+      | EXP_Bool    _
+      | EXP_Null
+      | EXP_Zero_initializer
+      | EXP_Cstring _
+      | EXP_Undef => e
+      | EXP_Struct fields =>
+        EXP_Struct _ (List.map (fun '(t,e) => (swap id1 id2 t, swap_exp id1 id2 e)) fields)
+      | EXP_Packed_struct fields =>
+        EXP_Packed_struct _ (List.map (fun '(t,e) => (swap id1 id2 t, swap_exp id1 id2 e)) fields)    
+      | EXP_Array elts =>
+        EXP_Array _ (List.map (fun '(t,e) => (swap id1 id2 t, swap_exp id1 id2 e)) elts)
+      | EXP_Vector elts =>
+        EXP_Vector _ (List.map (fun '(t,e) => (swap id1 id2 t, swap_exp id1 id2 e)) elts)
+      | OP_IBinop iop t v1 v2 =>
+        OP_IBinop _ (swap id1 id2 iop) (swap id1 id2 t) (swap_exp id1 id2 v1) (swap_exp id1 id2 v2)
+      | OP_ICmp cmp t v1 v2 =>
+        OP_ICmp _ (swap id1 id2 cmp) (swap id1 id2 t) (swap_exp id1 id2 v1) (swap_exp id1 id2 v2)
+      | OP_FBinop fop fm t v1 v2 =>
+        OP_FBinop _ (swap id1 id2 fop) fm (swap id1 id2 t) (swap_exp id1 id2 v1) (swap_exp id1 id2 v2)    
+      | OP_FCmp cmp t v1 v2 =>
+        OP_FCmp _ (swap id1 id2 cmp) (swap id1 id2 t) (swap_exp id1 id2 v1) (swap_exp id1 id2 v2)    
+      | OP_Conversion conv t_from v t_to =>
+        OP_Conversion _ conv (swap id1 id2 t_from) (swap_exp id1 id2 v) (swap id1 id2 t_to)
+      | OP_GetElementPtr t ptrval idxs =>
+        OP_GetElementPtr _ (swap id1 id2 t) (swap id1 id2 (fst ptrval), swap_exp id1 id2 (snd ptrval))
+                         (List.map (fun '(t,e) => (swap id1 id2 t, swap_exp id1 id2 e)) idxs)
+      | OP_ExtractElement vec idx =>
+        OP_ExtractElement _ (swap id1 id2 (fst vec), swap_exp id1 id2 (snd vec))
+                          (swap id1 id2 (fst idx), swap_exp id1 id2 (snd idx))
+      | OP_InsertElement  vec elt idx =>
+        OP_InsertElement _ (swap id1 id2 (fst vec), swap_exp id1 id2 (snd vec))
+                         (swap id1 id2 (fst elt), swap_exp id1 id2 (snd elt))                     
+                         (swap id1 id2 (fst idx), swap_exp id1 id2 (snd idx))
+      | OP_ShuffleVector vec1 vec2 idxmask =>
+        OP_ShuffleVector _ (swap id1 id2 (fst vec1), swap_exp id1 id2 (snd vec1))
+                         (swap id1 id2 (fst vec2), swap_exp id1 id2 (snd vec2))                     
+                         (swap id1 id2 (fst idxmask), swap_exp id1 id2 (snd idxmask))
+      | OP_ExtractValue  vec idxs =>
+        OP_ExtractValue  _ (swap id1 id2 (fst vec), swap_exp id1 id2 (snd vec))
+                         idxs
+      | OP_InsertValue vec elt idxs =>
+        OP_InsertValue _ (swap id1 id2 (fst vec), swap_exp id1 id2 (snd vec))
+                       (swap id1 id2 (fst elt), swap_exp id1 id2 (snd elt))
+                       idxs
+      | OP_Select cnd v1 v2 =>
+        OP_Select _ (swap id1 id2 (fst cnd), swap_exp id1 id2 (snd cnd))
+                  (swap id1 id2 (fst v1), swap_exp id1 id2 (snd v1))
+                  (swap id1 id2 (fst v2), swap_exp id1 id2 (snd v2))
+      end.
+
+    Global Instance swap_of_exp : Swap (exp T) := swap_exp.
+    Hint Unfold swap_of_exp.
+
+    Definition swap_instr_id (id1 id2:raw_id) (i:instr_id) : instr_id :=
+      match i with
+      | IId id => IId (swap id1 id2 id)
+      | IVoid n => IVoid n  (* TODO: support renaming these too? *)
+      end.
+
+    Global Instance swap_of_instr_id : Swap instr_id := swap_instr_id.
+    Hint Unfold swap_of_instr_id.
+
+    Definition swap_phi (id1 id2:raw_id) (p:phi T) : phi T :=
+      match p with
+      | Phi t args => Phi _ (swap id1 id2 t) (swap id1 id2 args)
+      end.
+    Global Instance swap_of_phi : Swap (phi T) := swap_phi.
+    Hint Unfold swap_of_phi.
+
+    Definition swap_instr (id1 id2:raw_id) (ins:instr T) : instr T :=
+      match ins with
+      | INSTR_Op op => INSTR_Op _ (swap id1 id2 op)
+      | INSTR_Call fn args => INSTR_Call _ (swap id1 id2 fn) (swap id1 id2 args)
+      | INSTR_Alloca t nb align =>
+        INSTR_Alloca _ (swap id1 id2 t) (swap id1 id2 nb) align
+      | INSTR_Load volatile t ptr align =>
+        INSTR_Load _ volatile (swap id1 id2 t) (swap id1 id2 ptr) align
+      | INSTR_Store volatile val ptr align =>
+        INSTR_Store _ volatile (swap id1 id2 val) (swap id1 id2 ptr) align
+      | INSTR_Comment _
+      | INSTR_Fence
+      | INSTR_AtomicCmpXchg
+      | INSTR_AtomicRMW
+      | INSTR_Unreachable
+      | INSTR_VAArg
+      | INSTR_LandingPad => ins
+      end.
+    Global Instance swap_of_instr : Swap (instr T) := swap_instr.
+    Hint Unfold swap_of_instr.
+
+    Definition swap_terminator (id1 id2:raw_id) (trm:terminator T) : terminator T :=
+      match trm with
+      | TERM_Ret  v => TERM_Ret _ (swap id1 id2 v)
+      | TERM_Ret_void => TERM_Ret_void _
+      | TERM_Br v br1 br2 => TERM_Br _ (swap id1 id2 v) (swap id1 id2 br1) (swap id1 id2 br2)
+      | TERM_Br_1 br => TERM_Br_1 _ (swap id1 id2 br)
+      | TERM_Switch  v default_dest brs =>
+        TERM_Switch _ (swap id1 id2 v) (swap id1 id2 default_dest) (swap id1 id2 brs)
+      | TERM_IndirectBr v brs =>
+        TERM_IndirectBr _ (swap id1 id2 v) (swap id1 id2 brs)
+      | TERM_Resume v => TERM_Resume _ (swap id1 id2 v)
+      | TERM_Invoke fnptrval args to_label unwind_label =>
+        TERM_Invoke _ (swap id1 id2 fnptrval) (swap id1 id2 args) (swap id1 id2 to_label) (swap id1 id2 unwind_label)
+      end.
+    Global Instance swap_of_terminator : Swap (terminator T) := swap_terminator.
+    Hint Unfold swap_of_terminator.
+
+    Global Instance swap_of_param_attr : Swap param_attr :=
+      fun id1 id2 l => l.
+    Global Instance swap_of_fn_attr : Swap fn_attr :=
+      fun id1 id2 l => l.
+    Global Instance swap_of_cconv : Swap cconv :=
+      fun id1 id2 l => l.
+    Global Instance swap_of_linkage : Swap linkage :=
+      fun id1 id2 l => l.
+    Global Instance swap_of_visibility : Swap visibility :=
+      fun id1 id2 l => l.
+    Global Instance swap_of_dll_storage : Swap dll_storage :=
+      fun id1 id2 l => l.
+    Global Instance swap_of_thread_local_storage : Swap thread_local_storage :=
+      fun id1 id2 l => l.
+
+    Hint Unfold swap_of_param_attr swap_of_fn_attr swap_of_cconv swap_of_linkage swap_of_visibility swap_of_dll_storage swap_of_thread_local_storage.
+
+    Definition swap_global (id1 id2:raw_id) (g:global T) : (global T) :=
+      mk_global _
+                (swap id1 id2 (g_ident _ g))
+                (swap id1 id2 (g_typ _ g))     
+                (swap id1 id2 (g_constant _ g))
+                (swap id1 id2 (g_exp _ g))
+                (swap id1 id2 (g_linkage _ g))
+                (swap id1 id2 (g_visibility _ g))
+                (swap id1 id2 (g_dll_storage _ g))
+                (swap id1 id2 (g_thread_local _ g))
+                (swap id1 id2 (g_unnamed_addr _ g))
+                (swap id1 id2 (g_addrspace _ g))
+                (swap id1 id2 (g_externally_initialized _ g))
+                (swap id1 id2 (g_section _ g))
+                (swap id1 id2 (g_align _ g)).
+    Hint Unfold swap_global.
+    Global Instance swap_of_global : Swap (global T) := swap_global.
+    Hint Unfold swap_of_global.
+
+    Definition swap_declaration (id1 id2:raw_id) (d:declaration T) : declaration T :=
+      mk_declaration _
+                     (swap id1 id2 (dc_name _ d))
+                     (swap id1 id2 (dc_type _ d))
+                     (swap id1 id2 (dc_param_attrs _ d))
+                     (swap id1 id2 (dc_linkage _ d))
+                     (swap id1 id2 (dc_visibility _ d))
+                     (swap id1 id2 (dc_dll_storage _ d))
+                     (swap id1 id2 (dc_cconv _ d))
+                     (swap id1 id2 (dc_attrs _ d))
+                     (swap id1 id2 (dc_section _ d))
+                     (swap id1 id2 (dc_align _ d))
+                     (swap id1 id2 (dc_gc _ d)).
+    Hint Unfold swap_declaration.
+    Global Instance swap_of_declaration : Swap (declaration T) := swap_declaration.    
+    Hint Unfold swap_of_declaration.
+
+    Definition swap_block (id1 id2:raw_id) (b:block T) : block T :=
+      mk_block _ (swap id1 id2 (blk_id _ b))
+               (swap id1 id2 (blk_phis _ b))
+               (swap id1 id2 (blk_code _ b))
+               (swap id1 id2 (blk_term _ b))
+               (blk_comments _ b).
+    Hint Unfold swap_block.  
+    Global Instance swap_of_block : Swap (block T) := swap_block.
+    Hint Unfold swap_of_block.
+
+    Definition swap_definition {FnBody:Set} `{SF: Swap FnBody} (id1 id2:raw_id) (d:definition T FnBody) : definition T FnBody :=
+      mk_definition _ _
+                    (swap id1 id2 (df_prototype _ _ d))
+                    (swap id1 id2 (df_args _ _ d))
+                    (swap id1 id2 (df_instrs _ _ d)).
+    Hint Unfold swap_definition.
+
+    Global Instance swap_of_definition {FnBody:Set} `{SF:Swap FnBody} : Swap (definition T FnBody) :=
+      swap_definition.
+    Hint Unfold swap_of_definition.
+
+
+    Fixpoint swap_metadata (id1 id2:raw_id) (m:metadata T) : metadata T :=
+      match m with
+      | METADATA_Const  tv => METADATA_Const _ (swap id1 id2 tv)
+      | METADATA_Null => METADATA_Null _
+      | METADATA_Id id => METADATA_Id _ (swap id1 id2 id)
+      | METADATA_String str => METADATA_String _ (swap id1 id2 str)
+      | METADATA_Named strs => METADATA_Named _ (swap id1 id2 strs)
+      | METADATA_Node mds => METADATA_Node _ (List.map (swap_metadata id1 id2) mds)
+      end.
+    Global Instance swap_of_metadata : Swap (metadata T) := swap_metadata.
+    Hint Unfold swap_of_metadata.
+
+    Definition swap_toplevel_entity {FnBody:Set} `{SF:Swap FnBody} (id1 id2:raw_id) (tle:toplevel_entity T FnBody) :=
+      match tle with
+      | TLE_Comment msg => tle
+      | TLE_Target tgt => TLE_Target _ _ (swap id1 id2 tgt)
+      | TLE_Datalayout layout => TLE_Datalayout _ _ (swap id1 id2 layout)
+      | TLE_Declaration decl => TLE_Declaration _ _ (swap id1 id2 decl)
+      | TLE_Definition defn => TLE_Definition _ _ (swap id1 id2 defn)
+      | TLE_Type_decl id t => TLE_Type_decl _ _ (swap id1 id2 id) (swap id1 id2 t)
+      | TLE_Source_filename s => TLE_Source_filename _ _ (swap id1 id2 s)
+      | TLE_Global g => TLE_Global _ _ (swap id1 id2 g)
+      | TLE_Metadata id md => TLE_Metadata _ _ (swap id1 id2 id) (swap id1 id2 md)
+      | TLE_Attribute_group i attrs => TLE_Attribute_group _ _ (swap id1 id2 i) (swap id1 id2 attrs)
+      end.
+
+    Global Instance swap_of_toplevel_entity {FnBody:Set} `{SF:Swap FnBody} : Swap (toplevel_entity T FnBody) :=
+      swap_toplevel_entity.
+    Hint Unfold swap_of_toplevel_entity.
+
+    Definition swap_modul {FnBody:Set} `{SF:Swap FnBody} (id1 id2:raw_id) (m:modul T FnBody) : modul T FnBody :=
+      mk_modul _ _
+               (swap id1 id2 (m_name _ _ m))
+               (swap id1 id2 (m_target _ _ m))
+               (swap id1 id2 (m_datalayout _ _ m))
+               (swap id1 id2 (m_type_defs _ _ m))
+               (swap id1 id2 (m_globals _ _ m))
+               (swap id1 id2 (m_declarations _ _ m))
+               (swap id1 id2 (m_definitions _ _ m)).
+    Hint Unfold swap_modul.
+
+    Global Instance swap_of_modul {FnBody:Set} `{SF:Swap FnBody} : Swap (modul T FnBody) :=
+      swap_modul.
+    Hint Unfold swap_of_modul.
+
+    Definition swap_cfg (id1 id2:raw_id) (CFG:cfg T) : cfg T :=
+      mkCFG _ (swap id1 id2 (init _ CFG)) (swap id1 id2 (blks _ CFG)) (swap id1 id2 (args _ CFG)).
+    Hint Unfold swap_cfg.
+
+    Global Instance swap_of_cfg : Swap (cfg T) := swap_cfg.
+    Hint Unfold swap_of_cfg.
+
+    Global Instance swap_of_mcfg : Swap (mcfg T) := swap.
+    Hint Unfold swap_of_mcfg.
+  End WithT.
+
+  (******************** Semantic swaps ********************)
+  (**
+     [GlobalE] and [LocalE] events depend on [raw_id]. The bisimulation between the denotation
+     of a MCFG and the one of its swapped version can therefore only be established after
+     interpretation of those.
+     However we first establish as an intermediate result that the denotation of the swapped
+     program, before any interpretation, results in the swapping of original denotation.
+   *)
+
+  Instance swap_of_inttyp : forall {x:Z}, Swap (inttyp x) := fun _ id1 id2 a => a.
+  Instance swap_of_int1 : Swap int1 := fun id1 id2 a => a.
+  Instance swap_of_int32 : Swap int32 := fun id1 id2 a => a.
+  Instance swap_of_int64 : Swap int64 := fun id1 id2 a => a.
+  Instance swap_of_ll_double : Swap ll_double := fun id1 id2 a => a.
+  Instance swap_of_ll_float : Swap ll_float := fun id1 id2 a => a.
+  Hint Unfold swap_of_inttyp swap_of_int1 swap_of_int32 swap_of_int64 swap_of_ll_double swap_of_ll_float.
+
+  Instance swap_of_dvalue : Swap dvalue := fun (id1 id2 : raw_id) dv => dv.
+  Hint Unfold swap_of_dvalue.
+
+  Program Instance swap_invariant_dvalue_inst : SwapInvariant dvalue := _.
+  Next Obligation.
+    constructor. intros. unfold swap. reflexivity.
+  Defined.  
+
+  Instance swap_invariant_of_list {X} `{SwapInvariant X}: SwapInvariant (list X).
   Proof.
-    intros.
-    apply ENVFacts.not_find_in_iff.
-    unfold not. intros H1.
-    apply (@ENVFacts.empty_in_iff X id).
-    apply Empty_Equals in H.
-    rewrite H. assumption.
+    constructor.
+    intros ? ? l; induction l as [| x l IH]; [reflexivity | cbn].
+    rewrite swap_invariant.
+    f_equal; auto.
   Qed.
-*)
-  Variable id1 id2 : raw_id.
-  
-  Lemma swap_raw_id_inj : forall (k j:raw_id), swap id1 id2 k = swap id1 id2 j -> k = j.
-  Proof.
-    intros.
-    unfold_swaps. unfold swap_raw_id in *.
-    simpl_ifs; unfold eqv, eqv_raw_id in *; subst; try reflexivity; try contradiction.
-  Qed.
+
+  Instance swap_of_GlobalE {X} : Swap (LLVMGEnvE X) :=
+    fun id1 id2 e =>
+      match e with
+      | GlobalWrite id v => GlobalWrite (swap id1 id2 id) v 
+      | GlobalRead id => GlobalRead (swap id1 id2 id)
+      end.
+  Instance swap_of_LocalE {X} : Swap (LLVMEnvE X) :=
+    fun id1 id2 e =>
+      match e with
+      | LocalWrite id v => LocalWrite (swap id1 id2 id) v 
+      | LocalRead id => LocalRead (swap id1 id2 id)
+      end.
+  Instance swap_of_StackE v {X} : Swap (StackE raw_id v X) :=
+    fun id1 id2 e =>
+      match e with
+      | StackPush args => StackPush (List.map (fun '(id,v) => (swap id1 id2 id, v)) args)
+      | StackPop => StackPop
+      end.
+  Instance swap_of_MemoryE {X} : Swap (MemoryE X) := fun id1 id2 x => x.
+  Instance swap_of_CallE {X} : Swap (CallE X) := fun id1 id2 x => x.
+  Instance swap_of_IntrinsicE {X} : Swap (IntrinsicE X) := fun id1 id2 x => x.
+  Instance swap_of_DebugE {X} : Swap (DebugE X) := fun id1 id2 x => x.
+  Instance swap_of_FailureE {X} : Swap (FailureE X) := fun id1 id2 x => x.
+  Hint Unfold swap_of_MemoryE swap_of_StackE swap_of_LocalE swap_of_GlobalE swap_of_CallE swap_of_IntrinsicE swap_of_DebugE FailureE.
+
+  Instance swap_of_sum' {X E F} `{Swap (E X)} `{Swap (F X)}: Swap ((E +' F) X) :=
+    fun id1 id2 ef =>
+      match ef with
+      | inl1 e => inl1 (swap id1 id2 e)
+      | inr1 f => inr1 (swap id1 id2 f)
+      end.
+
+  (* Slightly fishy: shouldn't we swap the events on the way? *)
+  (* Giving a shot at actually translating the events too *)
+  (* Still slightly weird: all intermediate computed values are not swapped. *)
+  Definition swap_LLVM {X E} `{Swap X} `{forall T, Swap (E T)} (id1 id2:raw_id) (t:LLVM E X) : LLVM E X :=
+    ITree.map (swap id1 id2) (@translate E E (fun T => swap id1 id2) _ t).
+  Instance swap_of_LLVM {X E} `{SX : Swap X} `{forall T, Swap (E T)}: Swap (LLVM E X) := swap_LLVM.
+  Hint Unfold swap_of_LLVM.
+
+  (* Should we swap the arguments? Not when used to create an itree *)
+  Instance swap_of_fun {A B} (* `{Swap A} *) `{Swap B}: Swap (A -> B) :=
+    fun id1 id2 f a => swap id1 id2 (f a).
+  Hint Unfold swap_of_fun.
+
+  (******************** Correctness ********************)
+
+  Section PROOFS.
+
+    Variable id1 id2 : raw_id.
+
+    (******************** Type classes ********************)
+
+    Class Commute_eq1 {A B: Type} `{Swap A} `{Swap B} (f: A -> B) :=
+      commute_eq1: forall a, swap id1 id2 (f a) = f (swap id1 id2 a).
+
+    Class Commute_eq_LLVM1 {E} {A B: Type} `{forall T, Swap (E T)} `{Swap A} `{Swap B} (f: A -> LLVM E B) :=
+      commute_eq_LLVM1: forall a, swap id1 id2 (f a) ≅ f (swap id1 id2 a).
+
+    Class Commute_eq2 {A B C: Type} `{Swap A} `{Swap B} `{Swap C} (f: A -> B -> C) :=
+      commute_eq2: forall a b, swap id1 id2 (f a b) = f (swap id1 id2 a) (swap id1 id2 b).
+
+    Class Commute_eq_LLVM2 {E} {A B C: Type} `{forall T, Swap (E T)} `{Swap A} `{Swap B} `{Swap C}
+          (f: A -> B -> LLVM E C) :=
+      commute_eq_LLVM2: forall a b, swap id1 id2 (f a b) ≅ f (swap id1 id2 a) (swap id1 id2 b).
+
+    (******************** Proofs ********************)
+
+    Lemma swap_trigger {E F: Type -> Type} `{E -< F} `{forall T, Swap (F T)} {X} `{Swap X} `{Swap (E X)}:
+      forall (e: E X), @ITree.trigger F X (@subevent E F _ _ (swap id1 id2 e)) = swap id1 id2 (trigger e).
+    Admitted.
+
+    Instance Commute_lookup_id: Commute_eq1 lookup_id.
+    Proof.
+      intros i.
+      unfold lookup_id.
+      destruct i; cbn;
+        rewrite <- (@swap_trigger _ _CFG _ _ dvalue _ _ _); reflexivity.
+    Qed.
+
+    Lemma bind_vis'_ {E F} `{E -< F} {X Y Z} (e: E X) (ek: X -> itree F Y) (k: Y -> itree F Z) :
+      ITree.bind (vis e ek) k ≅ vis e (fun x => ITree.bind (ek x) k).
+    Admitted.
+
+    (* Remark: somewhat surprisingly one cannot derive [Swap (E T)> from [Swap (F T)] *)
+    Instance swap_subevent {E F} `{E -< F} `{forall T, Swap (F T)} `{forall T, Swap (E T)} T:
+      Commute_eq1 (@subevent E F _ T).
+    Proof.
+      intros e.
+      unfold subevent.
+     
+
+
+    Instance Commute_raise {E} `{FailureE -< E} `{forall T, Swap (E T)} {X} `{SX: Swap X} :
+      Commute_eq_LLVM1 raise.
+    Proof.
+      intros s; simpl.
+      unfold raise.
+      unfold swap, swap_of_LLVM, swap_LLVM, Exception.throw, ITree.map.
+      rewrite translate_vis, bind_vis.
+ 
+      match goal with
+      | |- context [translate ?h] => set (foo := h)
+      end.
+    Admitted.
+
+    (*   apply eq_itree_Vis; intros []. *)
+    (* Qed. *)
+
+    Instance Commute_Ret {A} {E: Type -> Type} `{Swap A} `{forall T, Swap (E T)}: @Commute_eq_LLVM1 E A A _ _ _ (fun x => Ret x).
+    Proof.
+      intros ?.
+      unfold swap, swap_of_LLVM, swap_LLVM.
+      rewrite translate_ret, map_ret.
+      reflexivity.
+    Qed.
+
+    (* TODO: turn into an instance *)
+    (* Weird to have to assume [SwapInvariant Y]. In particular, is there any case where
+       we don't bind with X = Y?
+     *)
+    Lemma swap_bind {X Y E} `{SX : Swap X} `{SY : Swap Y} `{forall T, Swap (E T)} `{SIY : SwapInvariant Y} : 
+      forall (e : LLVM E Y) (k : Y -> LLVM E X),
+        swap id1 id2 (ITree.bind e k) ≅ ITree.bind (swap id1 id2 e) (fun y => swap id1 id2 (k y)).
+    Proof.
+      intros.
+      unfold swap at 1, swap_of_LLVM, swap_LLVM.
+      rewrite translate_bind,map_bind.
+      unfold swap at 7.
+      rewrite bind_map.
+      apply eq_itree_bind; [intros ? | reflexivity].
+      rewrite (swap_invariant _ _ a).
+      reflexivity.
+    Qed.
+
+    (* The setoid version would be more resilient, but is just too slow to use :( *)
+    Ltac commute_swap := rewrite commute_eq1 || rewrite Commute_Ret || rewrite commute_eq_LLVM1.
+    Ltac commute_swap' := setoid_rewrite commute_eq1 || setoid_rewrite Commute_Ret || setoid_rewrite commute_eq_LLVM1.
+    Ltac solver       := simpl; commute_swap; reflexivity.
+    Ltac solver'       := simpl; commute_swap'; reflexivity.
+
+    (* Annoying form, and impractical to use overall :( *)
+    Instance Commute_lift_err {E} `{FailureE -< E} {A B} `{SX: Swap A} `{SX: Swap B} a:
+      Commute_eq_LLVM1 (fun f => @lift_err A B _ _ f a).
+    Proof.
+      intros k; destruct a; simpl.
+      rewrite commute_eq_LLVM1; reflexivity.
+      reflexivity.
+    Qed.
+
+    Instance Commute_map_monad {E} {X Y} `{Swap X} `{Swap Y} `{forall T, Swap (E T)} `{SwapInvariant X} `{SwapInvariant Y}:
+      Commute_eq_LLVM2 (@map_monad (LLVM E) _ X Y).
+    Proof.
+      intros f l; induction l as [| b l IH].
+      - solver.
+      - simpl.
+        rewrite swap_bind.
+        apply eq_itree_bind; [intros ? |].
+        rewrite swap_bind, IH.
+        apply eq_itree_bind; [intros ? | reflexivity].
+        rewrite Commute_Ret, swap_invariant; reflexivity.
+        rewrite (swap_invariant _ _ b); reflexivity.
+    Qed.
+
+    (* This cannot hold before interpretation of [GlobalE] and [LocalE] since the effects themselves refer to [raw_id] *)
+    (* Unless we actually define swap over itree as both mapping swap _and_ translating it? *)
+    Instance Commute_denote_exp : Commute_eq_LLVM2 denote_exp.
+    Proof.
+      intros top e; revert top.
+      induction e using exp_ind'; intros top.
+      - solver.
+      - cbn.
+        destruct top as [[]|].
+        2:{
+          simpl.
+          unfold raise.
+          unfold Exception.throw.
+
+Notation swap' := (swap id1 id2).
+Lemma foo: forall A `{Swap A}, swap' = @swap A _ id1 id2.
+  reflexivity.
+Qed.
+
+Notation "'Vis (subeventb' E F H T e ')' k" := (Vis (@subevent E F H T e) k) (at level 12). 
+
+rewrite foo.
+Lemma foo: forall {E F} {H: E -< F} {T: Type} e k, vis e k = Vis (@subevent E F H T e) k.
+
+          unfold subevent.
+         
+          
+          Set Printing Implicit.
+          Instance ReSum_inr
+          rewrite (@Commute_raise _CFG _ _ _).
+        {
+          simpl.
+
+        try solver.
+        simpl.
+        (* lift_err *)
+        unfold lift_err.
+        match goal with
+        | |- context[match ?x with | _ => _ end] => destruct x
+        end;
+          solver.
+      - destruct top as [[]|]; solver. 
+      - destruct top as [[]|]; solver. 
+      - destruct b; solver.
+      - solver.
+      - destruct top; solver. 
+      - solver. 
+      - destruct top; solver.
+      - simpl denote_exp.
+        rewrite swap_bind.
+        apply eq_itree_bind; [intros ?; solver |].
+        rewrite Commute_map_monad.
+
+
+        admit.
+      - destruct top as [[]|]; try solver. 
+        simpl.
+        rewrite swap_bind.
+
+
+        (swap id1 id2 (map_monad (fun '(dt, ex) => denote_exp (Some dt) ex) fields))
+
+        (* map_monad *)
+        admit.
+      - (* map_monad *)
+        admit.
+      - (* map_monad *)
+        admit.
+      - cbn.
+        rewrite swap_bind.
+        rewrite IHe1.
+        apply eq_itree_bind; [intros ? | reflexivity].
+        rewrite swap_bind.
+        rewrite IHe2.
+        apply eq_itree_bind; [intros ? | reflexivity].
+        admit.
+      - simpl; rewrite swap_bind, IHe1.
+        setoid_rewrite swap_bind.
+        setoid_rewrite IHe2.
+        apply eq_itree_bind; [intros ? | reflexivity].
+        apply eq_itree_bind; [intros ? | reflexivity].
+        admit.
+      - simpl; rewrite swap_bind, IHe1.
+        setoid_rewrite swap_bind.
+        setoid_rewrite IHe2.
+        apply eq_itree_bind; [intros ? | reflexivity].
+        apply eq_itree_bind; [intros ? | reflexivity].
+        admit.
+      - simpl; rewrite swap_bind, IHe1.
+        setoid_rewrite swap_bind.
+        setoid_rewrite IHe2.
+        apply eq_itree_bind; [intros ? | reflexivity].
+        apply eq_itree_bind; [intros ? | reflexivity].
+        admit.
+      - simpl; rewrite swap_bind, IHe.
+        apply eq_itree_bind; [intros ? | reflexivity].
+        (* eval_conv *)
+        admit.
+      - destruct ptrval.
+        simpl.
+        rewrite swap_bind, IHe.
+        apply eq_itree_bind; [intros ? | reflexivity].
+        rewrite swap_bind.
+        admit.
+      - 
+
+      - 
+
+        match goal with
+        | |- context[match ?x with | _ => _ end] => destruct x eqn:H
+        end;
+          match goal with
+          | |- context[match ?x with | _ => _ end] => destruct x eqn:H'
+          end.
+        rewrite commute_eq_LLVM1.
+        
+
+          solver.
+ 
 
   (*
   Lemma swap_ENV_find : forall {X} `{SX : Swap X} (e:ENV.t X) (id:raw_id),
@@ -583,8 +809,8 @@ Section PROOFS.
       apply swap_raw_id_inj in e1. contradiction.
       apply H2.
   Qed.
-*)
-(*  
+   *)
+  (*  
   Lemma swap_lookup_env : forall {X} `{SX : Swap X} (e:ENV.t X) (id:raw_id),
       (lookup_env (swap id1 id2 e) (swap id1 id2 id) = swap id1 id2 (lookup_env e id)).
   Proof.
@@ -595,14 +821,7 @@ Section PROOFS.
     (* destruct (ENV.find id e); unfold_swaps; simpl; reflexivity. *)
   Admitted.
 
-  Lemma swap_lookup_id : forall (g:genv) (e:env) (i:ident),
-      lookup_id (swap id1 id2 g) (swap id1 id2 e) (swap id1 id2 i) = swap id1 id2 (lookup_id g e i).
-  Proof.
-    intros g e i.
-    unfold lookup_id.
-    destruct i; simpl; apply swap_lookup_env.
-  Qed.
-  
+ 
   Lemma swap_eval_i1_op : forall (iop:ibinop) (x y:inttyp 1),
       eval_int_op (swap id1 id2 iop) (swap id1 id2 x) (swap id1 id2 y) = swap id1 id2 (eval_int_op iop x y).
   Proof.
@@ -653,7 +872,7 @@ Section PROOFS.
     unfold_swaps.
     destruct (eval_icmp icmp v1 v2); reflexivity.
   Qed.
-*)
+   *)
   (*
   (* Before changing ITrees to records, we could prove _equality_ here.  Now we prove 
      only bisimulation?
@@ -755,7 +974,7 @@ Section PROOFS.
 
     - cbn. econstructor. 
       
-*)
+   *)
 (* Change to the ITree affected the way that errors need to be handled here. *)      
     
   Admitted.
@@ -786,11 +1005,55 @@ Section PROOFS.
       
     - unfold swap at 2. simpl.
       rewrite Trace.matchM. simpl.
-    *)
+   *)
     
   Admitted.    
 
-    *)
-End PROOFS.  
+   *)
+  End PROOFS.  
 End RENAMING.
 
+(* Scrap *)
+(*
+    (*
+  (* TODO: Add to Coq Library *)
+  Lemma Empty_Equals : forall {X} (e:ENV.t X), ENV.Empty e -> ENV.Equal (ENV.empty X) e.
+  Proof.
+    intros.
+    apply ENVFacts.Equal_mapsto_iff.
+    intros k x.
+    pose (H1 := H k x). clearbody H1.
+    split.
+    intros H2.
+    apply ENVFacts.empty_mapsto_iff in H2. contradiction.
+    intros. contradiction.
+  Qed.
+
+  (* TODO: Add to Coq Library *)
+  Lemma find_Empty_none : forall {X} (e:ENV.t X) (id:raw_id), ENV.Empty e -> ENV.find id e = None.
+  Proof.
+    intros.
+    apply ENVFacts.not_find_in_iff.
+    unfold not. intros H1.
+    apply (@ENVFacts.empty_in_iff X id).
+    apply Empty_Equals in H.
+    rewrite H. assumption.
+  Qed.
+     *)
+  (*
+(* Parameter fold : forall A: Type, (key -> elt -> A -> A) -> t elt -> A -> A. *)
+Definition swap_ENV {X} `{SX : Swap X} (id1 id2:raw_id) (m:ENV.t X) : ENV.t X :=
+  ENV.fold (fun k v n => ENV.add (swap id1 id2 k) (swap id1 id2 v) n) m (ENV.empty X).
+Hint Unfold swap_ENV.
+  *)
+
+
+    Lemma swap_raw_id_inj : forall (k j:raw_id), swap id1 id2 k = swap id1 id2 j -> k = j.
+    Proof.
+      intros.
+      unfold_swaps. unfold swap_raw_id in *.
+      simpl_ifs; unfold eqv, eqv_raw_id in *; subst; try reflexivity; try contradiction.
+    Qed.
+
+
+*)
